Pair_Graph/Pair_Graph_Specs.thy
@@ -1,6 +1,5 @@
 theory Pair_Graph_Specs
-(*Should call Pair_Graph_Specs *)
-  imports Awalk "HOL-Data_Structures.Map_Specs" "HOL-Data_Structures.Set_Specs"
+  imports Awalk "Map_Addons" "Set_Addons"
  begin
 
 section \<open>Locale for Executable Functions on Directed Graphs\<close>
@@ -31,22 +30,30 @@ locale Set_Choose = Set_Rec set_rec
 fixes sel ::"'m \<Rightarrow> 'a"
 assumes choose: "s \<noteq> (empty set_rec) \<Longrightarrow> (isin set_rec) s (sel s)"
 begin
-*)
+
 
 locale Set_Map = Set
   where set = t_set for t_set +
 fixes t_map ::"('a \<Rightarrow> 'a) \<Rightarrow> 'm \<Rightarrow> 'm"
 assumes map: "bij_betw f (t_set s) t  \<Longrightarrow> t_set (t_map f s) = t"
+*)
 
-
-locale Set_Choose = Set 
-  where set = t_set for t_set +
+locale Set_Choose = set: Set 
+  where set = t_set for t_set ("[_]\<^sub>s") +
 fixes sel ::"'m \<Rightarrow> 'a"
-assumes choose: "s \<noteq> empty \<Longrightarrow> isin s (sel s)"
+
+assumes choose [simp]: "s \<noteq> empty \<Longrightarrow> isin s (sel s)"
+
+
+begin
+context
+  includes set.automation
 begin
 
+(*
 declare set_empty[simp] set_isin[simp] set_insert[simp] set_delete[simp]
         invar_empty[simp] invar_insert[simp] invar_delete[simp] choose[simp]
+*)
 
 subsection \<open>Abstraction lemmas\<close>
 
@@ -55,25 +62,26 @@ text \<open>These are lemmas for automation. Their purpose is to remove any ment
 
 lemma choose'[simp, intro,dest]:
   "s \<noteq> empty \<Longrightarrow> invar s \<Longrightarrow> sel s \<in> t_set s"
-  by(auto simp flip: set_isin)
+  by(auto simp flip: set.set_isin)
 
 lemma choose''[intro]:
   "invar s \<Longrightarrow> s \<noteq> empty \<Longrightarrow> t_set s \<subseteq> s' \<Longrightarrow> sel s \<in> s'"
-  by(auto simp flip: set_isin)
+  by(auto simp flip: set.set_isin)
 
 lemma emptyD[dest]:
            "s = empty \<Longrightarrow> t_set s = {}"
            "s \<noteq> empty \<Longrightarrow> invar s \<Longrightarrow> t_set s \<noteq> {}"
            "empty = s \<Longrightarrow> t_set s = {}"
            "empty \<noteq> s \<Longrightarrow> invar s \<Longrightarrow> t_set s \<noteq> {}"
- using local.set_empty
+ using set.set_empty
  by auto
-
 end
-
+end
+(*
 locale Adj_Map_Specs = 
  adj: Map 
  where update = update and invar = adj_inv +
+
 
  neighb: Set_Choose
  where empty = neighb_empty and delete = neighb_delete and insert = neighb_insert and invar = neighb_inv
@@ -84,47 +92,108 @@ locale Adj_Map_Specs =
      neighb_empty :: "'neighb"  ("\<emptyset>\<^sub>N") and neighb_delete :: "'a \<Rightarrow> 'neighb \<Rightarrow> 'neighb" and
      neighb_insert and neighb_inv and isin
 
+
   \<comment> \<open>Why do we need ann efficient neghbourhood test?\<close>
 
+
 begin
+
+
+end
+*)
+
+no_notation digraph ("digraph")
+
+
+named_theorems Graph_Spec_Elims
+named_theorems Graph_Spec_Intros
+named_theorems Graph_Spec_Simps
+
+locale  Pair_Graph_Specs = 
+ adj: Map 
+ where update = update and invar = adj_inv +
+
+
+ neighb: Set_Choose
+ where empty = neighb_empty and delete = neighb_delete and invar = neighb_inv
+
+ for update :: "'v \<Rightarrow> 'neighb \<Rightarrow> 'adj \<Rightarrow> 'adj" and adj_inv :: "'adj \<Rightarrow> bool"  and
+
+     neighb_empty :: "'neighb" and neighb_delete :: "'v \<Rightarrow> 'neighb \<Rightarrow> 'neighb" and
+     neighb_inv
+(*  Adj_Map_Specs where update = update
+for update :: "'a \<Rightarrow> 'neighb \<Rightarrow> 'adj \<Rightarrow> 'adj"*) 
+begin
+
+notation neighb_empty ("\<emptyset>\<^sub>N")
+notation empty ("\<emptyset>\<^sub>G")
 
 abbreviation isin' (infixl "\<in>\<^sub>G" 50) where "isin' G v \<equiv> isin v G" 
 abbreviation not_isin' (infixl "\<notin>\<^sub>G" 50) where "not_isin' G v \<equiv> \<not> isin' G v"
 
 definition "set_of_map (m::'adj) \<equiv> {(u,v). case (lookup m u) of Some vs \<Rightarrow> v \<in>\<^sub>G vs}"
 
-end
-
-no_notation digraph ("digraph")
-
-locale  Pair_Graph_Specs = 
-  Adj_Map_Specs where update = update
-for update :: "'a \<Rightarrow> 'neighb \<Rightarrow> 'adj \<Rightarrow> 'adj" (*+
-fixes graph_inv:: "'adj \<Rightarrow> bool"
-
-assumes neighbourhood_invars:
- "graph_inv G \<Longrightarrow> adj_inv G"
- "\<lbrakk>graph_inv G; lookup G v = Some neighb\<rbrakk> \<Longrightarrow> neighb_inv neighb"
-
-   "adj_inv digraph" and
-   \<comment> \<open>This is because in the abstract graph model we have no disconnected vertices.\<close>
-   neighbourhood_invars:
-   "(lookup digraph v = Some neighb)"
-   "lookup digraph v = Some neighb \<Longrightarrow> neighb_inv neighb"
-
-assumes finite_neighbourhoods:
-        "finite {v. (lookup G v) \<noteq> None}"
-        "finite (t_set N)"*)
-
-begin
-
 definition "graph_inv G \<equiv> (adj_inv G \<and> (\<forall>v neighb. lookup G v = Some neighb \<longrightarrow> neighb_inv neighb))"
 definition "finite_graph G \<equiv> (finite {v. (lookup G v) \<noteq> None})"
 definition "finite_neighbs \<equiv> (\<forall>N. finite (t_set N))"
 
+
+definition neighbourhood::"'adj \<Rightarrow> 'v \<Rightarrow> 'neighb" where
+  "neighbourhood G v \<equiv> (case (lookup G v) of Some neighb \<Rightarrow> neighb | _ \<Rightarrow> neighb_empty)"
+
+notation "neighbourhood" ("\<N>\<^sub>G _ _" 100)
+
+definition digraph_abs ("[_]\<^sub>g") where "digraph_abs G \<equiv> {(u,v). v \<in>\<^sub>G (\<N>\<^sub>G G u)}" 
+
+definition "add_edge G u v \<equiv> 
+( 
+  case (lookup G u) of Some neighb \<Rightarrow> 
+  let
+    neighb = the (lookup G u);
+    neighb' = insert v neighb;
+    digraph' = update u neighb' G
+  in
+    digraph'
+  | _ \<Rightarrow>
+  let
+    neighb' = insert v neighb_empty;
+    digraph' = update u neighb' G
+  in
+    digraph'
+ 
+)"
+
+definition "delete_edge G u v \<equiv> 
+( 
+  case (lookup G u) of Some neighb \<Rightarrow> 
+  let
+    neighb = the (lookup G u);
+    neighb' = neighb_delete v neighb;
+    digraph' = update u neighb' G
+  in
+    digraph'
+  | _ \<Rightarrow> G 
+)"
+
+
+
+context \<comment>\<open>Locale properties\<close>
+  includes adj.automation neighb.set.automation
+  fixes G::'adj
+  (*assumes [simp]:"axioms G"*)
+begin
+
 lemma graph_invE[elim]: 
   "graph_inv G \<Longrightarrow> (\<lbrakk>adj_inv G; (\<And>v neighb. lookup G v = Some neighb \<Longrightarrow> neighb_inv neighb)\<rbrakk> \<Longrightarrow> P) \<Longrightarrow> P"
   by (auto simp: graph_inv_def)
+
+(*end*)
+
+(*context \<comment>\<open>Locale properties\<close>
+  includes automation
+  fixes G::'adj
+  (*assumes [simp]:"axioms G"*)
+begin*)
 
 lemma graph_invI[intro]: 
   "\<lbrakk>adj_inv G; (\<And>v neighb. lookup G v = Some neighb \<Longrightarrow> neighb_inv neighb)\<rbrakk> \<Longrightarrow> graph_inv G"
@@ -146,22 +215,11 @@ lemma finite_neighbsI[intro]:
   "(\<And>N. finite (t_set N)) \<Longrightarrow> finite_neighbs"
   by (auto simp: finite_neighbs_def)
 
-declare adj.map_empty[simp] adj.map_update[simp] adj.map_delete[simp] adj.invar_empty[simp]
-        adj.invar_update[simp] adj.invar_delete[simp]
-
-declare neighb.set_empty[simp] neighb.set_isin[simp] neighb.set_insert[simp] neighb.set_delete[simp]
-        neighb.invar_empty[simp] neighb.invar_insert[simp] neighb.invar_delete[simp] neighb.choose[simp]
-
-definition neighbourhood::"'adj \<Rightarrow> 'a \<Rightarrow> 'neighb" where
-  "neighbourhood G v \<equiv> (case (lookup G v) of Some neighb \<Rightarrow> neighb | _ \<Rightarrow> neighb_empty)"
-
-notation "neighbourhood" ("\<N>\<^sub>G _ _" 100)
 
 lemma neighbourhood_invars'[simp,dest]:
    "graph_inv G \<Longrightarrow> neighb_inv (\<N>\<^sub>G G v)"
   by (auto simp add: graph_inv_def neighbourhood_def split: option.splits)
 
-definition "digraph_abs G \<equiv> {(u,v). v \<in>\<^sub>G (\<N>\<^sub>G G u)}"
 
 lemma finite_graph[intro!]:
   assumes "graph_inv G" "finite_graph G" "finite_neighbs"
@@ -214,48 +272,18 @@ lemma are_connected_absI[intro]:
 
 lemma neighbourhood_absD[dest!]:
   "\<lbrakk>t_set (\<N>\<^sub>G G x) \<noteq> {}; graph_inv G\<rbrakk> \<Longrightarrow> x \<in> dVs (digraph_abs G)"
-  by (auto simp: dVs_def dest!: neighb.emptyD)
+  by blast
 
 lemma neighbourhood_abs[simp]:
   "graph_inv G \<Longrightarrow> t_set (\<N>\<^sub>G G u) = Pair_Graph.neighbourhood (digraph_abs G) u"
   by(auto simp: digraph_abs_def neighbourhood_def Pair_Graph.neighbourhood_def option.discI graph_inv_def
           split: option.split)
 
-definition "add_edge G u v \<equiv> 
-( 
-  case (lookup G u) of Some neighb \<Rightarrow> 
-  let
-    neighb = the (lookup G u);
-    neighb' = neighb_insert v neighb;
-    digraph' = update u neighb' G
-  in
-    digraph'
-  | _ \<Rightarrow>
-  let
-    neighb' = neighb_insert v neighb_empty;
-    digraph' = update u neighb' G
-  in
-    digraph'
- 
-)"
-
 lemma adj_inv_insert[intro]: "graph_inv G \<Longrightarrow> graph_inv (add_edge G u v)"
   by (auto simp: add_edge_def graph_inv_def split: option.splits)
 
-lemma digraph_abs_insert[simp]: "graph_inv G \<Longrightarrow> digraph_abs (add_edge G u v) = insert (u,v) (digraph_abs G)"
+lemma digraph_abs_insert[simp]: "graph_inv G \<Longrightarrow> digraph_abs (add_edge G u v) = Set.insert (u,v) (digraph_abs G)"
   by (fastforce simp add: digraph_abs_def set_of_map_def neighbourhood_def add_edge_def split: option.splits if_splits)
-
-definition "delete_edge G u v \<equiv> 
-( 
-  case (lookup G u) of Some neighb \<Rightarrow> 
-  let
-    neighb = the (lookup G u);
-    neighb' = neighb_delete v neighb;
-    digraph' = update u neighb' G
-  in
-    digraph'
-  | _ \<Rightarrow> G 
-)"
 
 lemma adj_inv_delete[intro]: "graph_inv G \<Longrightarrow> graph_inv (delete_edge G u v)"
   by (auto simp: delete_edge_def graph_inv_def split: option.splits)
@@ -263,6 +291,12 @@ lemma adj_inv_delete[intro]: "graph_inv G \<Longrightarrow> graph_inv (delete_ed
 lemma digraph_abs_delete[simp]:  "graph_inv G \<Longrightarrow> digraph_abs (delete_edge G u v) = (digraph_abs G) - {(u,v)}"
   by (fastforce simp add: digraph_abs_def set_of_map_def neighbourhood_def delete_edge_def split: option.splits if_splits)
 
-end  
+
+end \<comment> \<open>Properties context\<close>  
+
+end text \<open>@{const Pair_Graph_Specs}\<close>
+
+
+
 
 end
