Pair_Graph/DFS_AVL.thy
@@ -1,0 +1,24 @@
+theory DFS_AVL
+  imports DFS Pair_Graph_AVL
+begin
+
+interpretation DFS_AVL: DFS
+  where empty=AVL_Set_Code.empty and update=update and delete = AVL_Map.delete and
+        lookup =lookup and adj_inv = M.invar  and neighb_empty = AVL_Set_Code.empty and 
+        neighb_insert = insert and neighb_delete = AVL_Set_Code.delete and isin = isin and 
+        t_set = "set o inorder" and neighb_inv = S.invar and sel = avl_sel 
+  apply(simp add: DFS_def)
+  apply(intro conjI)
+  subgoal using G.Pair_Graph_Specs_axioms .
+  subgoal sorry 
+  subgoal apply unfold_locales 
+    subgoal apply(auto simp: G.graph_inv_def)
+
+(* subgoal  apply unfold_locales
+    apply(simp add: M.invar_def)
+    by (metis avl_fold_works avl_map_dom_inorder)
+  done*)
+  done
+
+
+end
