Pair_Graph/Pair_Graph_AVL.thy
@@ -6,10 +6,8 @@ fun avl_sel where
   "avl_sel Leaf = undefined"
 | "avl_sel (Node _ (a,_) _) = a"
 
-lemma avl_sel_works: "(set o inorder) t \<noteq> {} \<Longrightarrow> avl_sel t \<in> (set o inorder) t"
-  by (induction t) auto
-
-thm S.invar_def
+lemma avl_sel_works: "t \<noteq> empty \<Longrightarrow> avl_sel t \<in> (set o inorder) t"
+  by (induction t) (auto simp: empty_def)
 
 fun avl_fold_keys::"('a \<Rightarrow> 'b \<Rightarrow> 'b) \<Rightarrow> (('a \<times> 'd) \<times> 'c) tree \<Rightarrow> 'b \<Rightarrow> 'b" where
   "avl_fold_keys f Leaf acc = acc"
@@ -27,30 +25,37 @@ lemma avl_map_dom_inorder: "sorted1 (inorder m) \<Longrightarrow> dom (lookup m)
   by (metis dom_map_of_fst ext)
 
 interpretation S_C: Set_Choose 
-
 where empty = AVL_Set_Code.empty and insert = insert and delete = AVL_Set_Code.delete and
       isin = isin and t_set = "set o inorder" and invar = S.invar and sel = avl_sel
   apply(simp add: Set_Choose_def)
   apply(intro conjI)
   subgoal using S.Set_axioms[unfolded] by(auto simp add: S.set_def S.invar_def)
-  subgoal using avl_sel_works by unfold_locales auto
+  subgoal apply unfold_locales subgoal for s by (cases s)  (auto dest!: avl_sel_works)
+  done
   done
 
-find_theorems name: S_C
 interpretation G: Adj_Map_Specs
   where empty=AVL_Set_Code.empty and update=update and delete = AVL_Map.delete and
         lookup =lookup and adj_inv = M.invar  and neighb_empty = AVL_Set_Code.empty and 
         neighb_insert = insert and neighb_delete = AVL_Set_Code.delete and isin = isin and 
-        t_set = "set o inorder" and neighb_inv = S.invar and sel = avl_sel and
-        adj_foreach = avl_fold_keys
+        t_set = "set o inorder" and neighb_inv = S.invar and sel = avl_sel 
   apply(simp add: Adj_Map_Specs_def)
   apply(intro conjI)
   subgoal using M.Map_axioms .
   subgoal using S_C.Set_Choose_axioms .
-  subgoal 
-  apply unfold_locales
+(* subgoal  apply unfold_locales
     apply(simp add: M.invar_def)
     by (metis avl_fold_works avl_map_dom_inorder)
+  done*)
   done
+
+interpretation G: Pair_Graph_Specs
+  where empty=AVL_Set_Code.empty and update=update and delete = AVL_Map.delete and
+        lookup =lookup and adj_inv = M.invar  and neighb_empty = AVL_Set_Code.empty and 
+        neighb_insert = insert and neighb_delete = AVL_Set_Code.delete and isin = isin and 
+        t_set = "set o inorder" and neighb_inv = S.invar and sel = avl_sel 
+  apply(simp add: Pair_Graph_Specs_def)
+  using G.Adj_Map_Specs_axioms
+  .
 
 end
